coq/Compiler/Driver/CompLang.v
@@ -35,6 +35,7 @@ Require Import NRARuntime.
 Require Import NRAEnvRuntime.
 Require Import NNRCRuntime.
 Require Import NNRCimpishRuntime.
+Require Import NNRCimpRuntime.
 Require Import NNRCMRRuntime.
 Require Import CldMRRuntime.
 Require Import DNNRCRuntime.
@@ -69,6 +70,7 @@ Section CompLang.
     | L_nnrc : language
     | L_nnrc_impish_core : language
     | L_nnrc_impish : language
+    | L_nnrc_imp : language
     | L_nnrcmr : language
     | L_cldmr : language
     | L_dnnrc : language
@@ -115,6 +117,7 @@ Section CompLang.
       | "nnrc"%string => L_nnrc
       | "nnrc_impish_core"%string => L_nnrc_impish_core
       | "nnrc_impish"%string => L_nnrc_impish
+      | "nnrc_imp"%string => L_nnrc_imp
       | "nnrcmr"%string => L_nnrcmr
       | "cldmr"%string => L_cldmr
       | "dnnrc"%string => L_dnnrc
@@ -146,6 +149,7 @@ Section CompLang.
       | L_nnrc => "nnrc"%string
       | L_nnrc_impish_core => "nnrc_impish_core"%string
       | L_nnrc_impish => "nnrc_impish"%string
+      | L_nnrc_imp => "nnrc_imp"%string
       | L_nnrcmr => "nnrcmr"%string
       | L_cldmr => "cldmr"%string
       | L_dnnrc => "dnnrc"%string
@@ -207,6 +211,7 @@ Section CompLang.
         :: (L_nnrc,CoreEnd,"NNRC", "Named Nested Relational Calculus")
         :: (L_nnrc_impish_core,BackEnd,"cNNRCimpish", "Core Named Nested Relational Calculus imperative")
         :: (L_nnrc_impish,BackEnd,"NNRCimpish", "Named Nested Relational Calculus imperative")
+        :: (L_nnrc_imp,BackEnd,"NNRCimp", "Named Nested Relational Calculus imperative")
         :: (L_nnrcmr,DistrEnd,"NNRCMR", "Named Nested Relational Calculus with Map/Reduce")
         :: (L_cldmr,DistrEnd,"CldMR", "Named Nested Relational Calculus with Cloudant Map/Reduce")
         :: (L_dnnrc,DistrEnd,"DNNRC", "Distributed Named Nested Relational Calculus")
@@ -299,6 +304,7 @@ Section CompLang.
     Definition nnrc := nnrc.
     Definition nnrc_impish_core := nnrc_impish_core.
     Definition nnrc_impish := nnrc_impish.
+    Definition nnrc_imp := nnrc_imp.
     Definition nnrcmr := nnrcmr.
     Definition cldmr := cldmr.
     Definition dnnrc := dnnrc.
@@ -326,6 +332,7 @@ Section CompLang.
     | Q_nnrc : nnrc -> query
     | Q_nnrc_impish_core : nnrc_impish_core -> query
     | Q_nnrc_impish : nnrc_impish -> query
+    | Q_nnrc_imp : nnrc_imp -> query
     | Q_nnrcmr : nnrcmr -> query
     | Q_cldmr : cldmr -> query
     | Q_dnnrc : dnnrc -> query
@@ -355,6 +362,7 @@ Section CompLang.
       | Case_aux c "Q_nnrc"%string
       | Case_aux c "Q_nnrc_impish_core"%string
       | Case_aux c "Q_nnrc_impish"%string
+      | Case_aux c "Q_nnrc_imp"%string
       | Case_aux c "Q_nnrcmr"%string
       | Case_aux c "Q_cldmr"%string
       | Case_aux c "Q_dnnrc"%string
@@ -384,6 +392,7 @@ Section CompLang.
       | Q_nnrc _ => L_nnrc
       | Q_nnrc_impish_core _ => L_nnrc_impish_core
       | Q_nnrc_impish _ => L_nnrc_impish
+      | Q_nnrc_imp _ => L_nnrc_imp
       | Q_nnrcmr _ => L_nnrcmr
       | Q_cldmr _ => L_cldmr
       | Q_dnnrc _ => L_dnnrc
@@ -419,6 +428,7 @@ Section CompLang.
       | L_nnrc => nnrc
       | L_nnrc_impish_core => nnrc_impish_core
       | L_nnrc_impish => nnrc_impish
+      | L_nnrc_imp => nnrc_imp
       | L_nnrcmr => nnrcmr
       | L_cldmr => cldmr
       | L_dnnrc => dnnrc
@@ -452,6 +462,7 @@ Tactic Notation "language_cases" tactic(first) ident(c) :=
   | Case_aux c "L_nnrc"%string
   | Case_aux c "L_nnrc_impish_core"%string
   | Case_aux c "L_nnrc_impish"%string
+  | Case_aux c "L_nnrc_imp"%string
   | Case_aux c "L_nnrcmr"%string
   | Case_aux c "L_cldmr"%string
   | Case_aux c "L_dnnrc"%string
