coq/Compiler/Driver/CompDriver.v
@@ -36,6 +36,7 @@ Require Import NRARuntime.
 Require Import NRAEnvRuntime.
 Require Import NNRCRuntime.
 Require Import NNRCimpishRuntime.
+Require Import NNRCimpRuntime.
 Require Import NNRCMRRuntime.
 Require Import CldMRRuntime.
 Require Import DNNRCRuntime.
@@ -69,7 +70,8 @@ Require Import NRAEnvtocNRAEnv.
 Require Import NRAtocNRAEnv.
 Require Import NNRCtocNNRC.
 Require Import NNRCtoNNRCimpish.
-Require Import NNRCimpishtoJavaScriptAst.
+Require Import NNRCimpishtoNNRCimp.
+Require Import NNRCimptoJavaScriptAst.
 Require Import JavaScriptAsttoJavaScript.
 Require Import NNRCtoDNNRC.
 Require Import NNRCtoNNRCMR.
@@ -227,8 +229,11 @@ Section CompDriver.
     Definition nnrc_to_nnrc_impish (inputs: list var) (q: nnrc) : nnrc_impish :=
       nnrc_to_nnrc_impish_top inputs q.
 
-    Definition nnrc_impish_to_js_ast (inputs: list var) (q: nnrc_impish) : js_ast :=
-      nnrc_impish_to_js_ast_top inputs q.
+    Definition nnrc_impish_to_nnrc_imp (q: nnrc_impish) : nnrc_imp :=
+      nnrc_impish_to_nnrc_imp q.
+
+    Definition nnrc_imp_to_js_ast (inputs: list var) (q: nnrc_imp) : js_ast :=
+      nnrc_imp_to_js_ast_top inputs q.
 
     Definition js_ast_to_javascript (q: js_ast) : javascript :=
       js_ast_to_js_top q.
@@ -337,9 +342,14 @@ Section CompDriver.
     | Dv_dnnrc_to_dnnrc_typed : tdbindings -> dnnrc_typed_driver -> dnnrc_driver
   .
 
+  Inductive nnrc_imp_driver : Set :=
+    | Dv_nnrc_imp_stop : nnrc_imp_driver
+    | Dv_nnrc_imp_to_js_ast : (* inputs *) list var -> js_ast_driver -> nnrc_imp_driver
+  .
+
   Inductive nnrc_impish_driver : Set :=
     | Dv_nnrc_impish_stop : nnrc_impish_driver
-    | Dv_nnrc_impish_to_js_ast : (* inputs *) list var -> js_ast_driver -> nnrc_impish_driver
+    | Dv_nnrc_impish_to_nnrc_imp : nnrc_imp_driver -> nnrc_impish_driver
   .
 
   Inductive nnrc_impish_core_driver : Set :=
@@ -464,6 +474,7 @@ Section CompDriver.
   | Dv_nnrc : nnrc_driver -> driver
   | Dv_nnrc_impish_core : nnrc_impish_core_driver -> driver
   | Dv_nnrc_impish : nnrc_impish_driver -> driver
+  | Dv_nnrc_imp : nnrc_imp_driver -> driver
   | Dv_nnrcmr : nnrcmr_driver -> driver
   | Dv_cldmr : cldmr_driver -> driver
   | Dv_dnnrc : dnnrc_driver -> driver
@@ -493,6 +504,7 @@ Section CompDriver.
     | Case_aux c "Dv_nnrc"%string
     | Case_aux c "Dv_nnrc_impish_core"%string
     | Case_aux c "Dv_nnrc_impish"%string
+    | Case_aux c "Dv_nnrc_imp"%string
     | Case_aux c "Dv_nnrcmr"%string
     | Case_aux c "Dv_cldmr"%string
     | Case_aux c "Dv_dnnrc"%string
@@ -518,6 +530,7 @@ Section CompDriver.
     | Dv_nnrc _ => L_nnrc
     | Dv_nnrc_impish_core _ => L_nnrc_impish_core
     | Dv_nnrc_impish _ => L_nnrc_impish
+    | Dv_nnrc_imp _ => L_nnrc_imp
     | Dv_nnrcmr _ => L_nnrcmr
     | Dv_camp_rule _ => L_camp_rule
     | Dv_tech_rule _ => L_tech_rule
@@ -579,10 +592,16 @@ Section CompDriver.
     | Dv_cldmr_to_cloudant queryname h dv => 1 + driver_length_cloudant dv
     end.
 
+  Definition driver_length_nnrc_imp (dv: nnrc_imp_driver) :=
+    match dv with
+    | Dv_nnrc_imp_stop => 1
+    | Dv_nnrc_imp_to_js_ast _ dv => 1 + driver_length_js_ast dv
+    end.
+
   Definition driver_length_nnrc_impish (dv: nnrc_impish_driver) :=
     match dv with
     | Dv_nnrc_impish_stop => 1
-    | Dv_nnrc_impish_to_js_ast _ dv => 1 + driver_length_js_ast dv
+    | Dv_nnrc_impish_to_nnrc_imp dv => 1 + driver_length_nnrc_imp dv
     end.
 
   Definition driver_length_nnrc_impish_core (dv: nnrc_impish_core_driver) :=
@@ -724,6 +743,7 @@ Section CompDriver.
     | Dv_nnrc dv => driver_length_nnrc dv
     | Dv_nnrc_impish_core dv => driver_length_nnrc_impish_core dv
     | Dv_nnrc_impish dv => driver_length_nnrc_impish dv
+    | Dv_nnrc_imp dv => driver_length_nnrc_imp dv
     | Dv_nnrcmr dv => driver_length_nnrcmr dv
     | Dv_cldmr dv => driver_length_cldmr dv
     | Dv_dnnrc dv => driver_length_dnnrc dv
@@ -803,13 +823,24 @@ Section CompDriver.
       in
       (Q_cldmr q) :: queries.
 
+    Definition compile_nnrc_imp (dv: nnrc_imp_driver) (q: nnrc_imp) : list query :=
+      let queries :=
+          match dv with
+          | Dv_nnrc_imp_stop => nil
+          | Dv_nnrc_imp_to_js_ast inputs dv =>
+            let q := nnrc_imp_to_js_ast inputs q in
+            compile_js_ast dv q
+          end
+      in
+      (Q_nnrc_imp q) :: queries.
+
     Definition compile_nnrc_impish (dv: nnrc_impish_driver) (q: nnrc_impish) : list query :=
       let queries :=
           match dv with
           | Dv_nnrc_impish_stop => nil
-          | Dv_nnrc_impish_to_js_ast inputs dv =>
-            let q := nnrc_impish_to_js_ast inputs q in
-            compile_js_ast dv q
+          | Dv_nnrc_impish_to_nnrc_imp dv =>
+            let q := nnrc_impish_to_nnrc_imp q in
+            compile_nnrc_imp dv q
           end
       in
       (Q_nnrc_impish q) :: queries.
@@ -1087,6 +1118,7 @@ Section CompDriver.
       | (Dv_nnrc dv, Q_nnrc q) => compile_nnrc dv q
       | (Dv_nnrc_impish_core dv, Q_nnrc_impish_core q) => compile_nnrc_impish_core dv q
       | (Dv_nnrc_impish dv, Q_nnrc_impish q) => compile_nnrc_impish dv q
+      | (Dv_nnrc_imp dv, Q_nnrc_imp q) => compile_nnrc_imp dv q
       | (Dv_nnrcmr dv, Q_nnrcmr q) => compile_nnrcmr dv q
       | (Dv_cldmr dv, Q_cldmr q) => compile_cldmr dv q
       | (Dv_dnnrc dv, Q_dnnrc q) => compile_dnnrc dv q
@@ -1124,6 +1156,7 @@ Section CompDriver.
       | Dv_nnrc _
       | Dv_nnrc_impish_core _
       | Dv_nnrc_impish _
+      | Dv_nnrc_imp _
       | Dv_nnrcmr _
       | Dv_cldmr _
       | Dv_dnnrc _
@@ -1155,6 +1188,7 @@ Section CompDriver.
       | Dv_nnrc _
       | Dv_nnrc_impish_core _
       | Dv_nnrc_impish _
+      | Dv_nnrc_imp _
       | Dv_nnrcmr _
       | Dv_cldmr _
       | Dv_dnnrc _
@@ -1186,6 +1220,7 @@ Section CompDriver.
       | Dv_nnrc _
       | Dv_nnrc_impish_core _
       | Dv_nnrc_impish _
+      | Dv_nnrc_imp _
       | Dv_nnrcmr _
       | Dv_cldmr _
       | Dv_dnnrc _
@@ -1217,6 +1252,7 @@ Section CompDriver.
       | Dv_nnrc _
       | Dv_nnrc_impish_core _
       | Dv_nnrc_impish _
+      | Dv_nnrc_imp _
       | Dv_nnrcmr _
       | Dv_cldmr _
       | Dv_dnnrc _
@@ -1248,6 +1284,7 @@ Section CompDriver.
       | Dv_nnrc _
       | Dv_nnrc_impish_core _
       | Dv_nnrc_impish _
+      | Dv_nnrc_imp _
       | Dv_nnrcmr _
       | Dv_cldmr _
       | Dv_dnnrc _
@@ -1279,6 +1316,7 @@ Section CompDriver.
       | Dv_nnrc _
       | Dv_nnrc_impish_core _
       | Dv_nnrc_impish _
+      | Dv_nnrc_imp _
       | Dv_nnrcmr _
       | Dv_cldmr _
       | Dv_dnnrc _
@@ -1310,6 +1348,7 @@ Section CompDriver.
       | Dv_nnrc _
       | Dv_nnrc_impish_core _
       | Dv_nnrc_impish _
+      | Dv_nnrc_imp _
       | Dv_nnrcmr _
       | Dv_cldmr _
       | Dv_dnnrc _
@@ -1341,6 +1380,7 @@ Section CompDriver.
       | Dv_nnrc _
       | Dv_nnrc_impish_core _
       | Dv_nnrc_impish _
+      | Dv_nnrc_imp _
       | Dv_nnrcmr _
       | Dv_cldmr _
       | Dv_dnnrc _
@@ -1372,6 +1412,7 @@ Section CompDriver.
       | Dv_nnrc _
       | Dv_nnrc_impish_core _
       | Dv_nnrc_impish _
+      | Dv_nnrc_imp _
       | Dv_nnrcmr _
       | Dv_cldmr _
       | Dv_dnnrc _
@@ -1403,6 +1444,7 @@ Section CompDriver.
       | Dv_nnrc _
       | Dv_nnrc_impish_core _
       | Dv_nnrc_impish _
+      | Dv_nnrc_imp _
       | Dv_nnrcmr _
       | Dv_cldmr _
       | Dv_dnnrc _
@@ -1434,6 +1476,7 @@ Section CompDriver.
       | Dv_lambda_nra _
       | Dv_nnrc_impish_core _
       | Dv_nnrc_impish _
+      | Dv_nnrc_imp _
       | Dv_nnrcmr _
       | Dv_cldmr _
       | Dv_dnnrc _
@@ -1456,6 +1499,7 @@ Section CompDriver.
       | Dv_nnrc_core _
       | Dv_nraenv _
       | Dv_nnrc_impish _
+      | Dv_nnrc_imp _
       | Dv_nnrcmr _
       | Dv_dnnrc _
       | Dv_js_ast _
@@ -1498,6 +1542,7 @@ Section CompDriver.
       | Dv_sqlpp _
       | Dv_lambda_nra _
       | Dv_nnrc_impish_core _
+      | Dv_nnrc_imp _
       | Dv_js_ast _
       | Dv_nra _
       | Dv_nraenv_core _
@@ -1527,6 +1572,7 @@ Section CompDriver.
       | Dv_nnrc_core _
       | Dv_nnrc _
       | Dv_nnrc_impish_core _
+      | Dv_nnrc_imp _
       | Dv_nnrcmr _
       | Dv_cldmr _
       | Dv_dnnrc _
@@ -1543,7 +1589,7 @@ Section CompDriver.
       end
     | L_nnrc_impish =>
       match dv with
-      | Dv_js_ast dv => Dv_nnrc_impish (Dv_nnrc_impish_to_js_ast (vars_of_constants_config config.(comp_constants)) dv)
+      | Dv_nnrc_imp dv => Dv_nnrc_impish (Dv_nnrc_impish_to_nnrc_imp dv)
       | Dv_camp _
       | Dv_nraenv_core _
       | Dv_nraenv _
@@ -1559,6 +1605,39 @@ Section CompDriver.
       | Dv_nnrc _
       | Dv_nnrc_impish_core _
       | Dv_nnrc_impish _
+      | Dv_js_ast _
+      | Dv_nnrcmr _
+      | Dv_cldmr _
+      | Dv_dnnrc _
+      | Dv_dnnrc_typed _
+      | Dv_javascript _
+      | Dv_java _
+      | Dv_spark_rdd _
+      | Dv_spark_df _
+      | Dv_cloudant _ =>
+          Dv_error ("No compilation path from "++(name_of_language lang)++" to "++(name_of_driver dv))
+      | Dv_error err =>
+          Dv_error ("Cannot compile to error ("++err++")")
+      end
+    | L_nnrc_imp =>
+      match dv with
+      | Dv_js_ast dv => Dv_nnrc_imp (Dv_nnrc_imp_to_js_ast (vars_of_constants_config config.(comp_constants)) dv)
+      | Dv_camp _
+      | Dv_nraenv_core _
+      | Dv_nraenv _
+      | Dv_nra _
+      | Dv_camp_rule _
+      | Dv_tech_rule _
+      | Dv_designer_rule _
+      | Dv_oql _
+      | Dv_sql _
+      | Dv_sqlpp _
+      | Dv_lambda_nra _
+      | Dv_nnrc_core _
+      | Dv_nnrc _
+      | Dv_nnrc_impish_core _
+      | Dv_nnrc_impish _
+      | Dv_nnrc_imp _
       | Dv_nnrcmr _
       | Dv_cldmr _
       | Dv_dnnrc _
@@ -1583,6 +1662,7 @@ Section CompDriver.
       | Dv_nnrc_core _
       | Dv_nnrc_impish_core _
       | Dv_nnrc_impish _
+      | Dv_nnrc_imp _
       | Dv_camp_rule _
       | Dv_tech_rule _
       | Dv_designer_rule _
@@ -1621,6 +1701,7 @@ Section CompDriver.
       | Dv_nnrc _
       | Dv_nnrc_impish_core _
       | Dv_nnrc_impish _
+      | Dv_nnrc_imp _
       | Dv_nnrcmr _
       | Dv_cldmr _
       | Dv_dnnrc _
@@ -1654,6 +1735,7 @@ Section CompDriver.
       | Dv_nnrc _
       | Dv_nnrc_impish_core _
       | Dv_nnrc_impish _
+      | Dv_nnrc_imp _
       | Dv_nnrcmr _
       | Dv_cldmr _
       | Dv_js_ast _
@@ -1687,6 +1769,7 @@ Section CompDriver.
       | Dv_nnrc _
       | Dv_nnrc_impish_core _
       | Dv_nnrc_impish _
+      | Dv_nnrc_imp _
       | Dv_nnrcmr _
       | Dv_cldmr _
       | Dv_dnnrc _
@@ -1718,6 +1801,7 @@ Section CompDriver.
       | Dv_nnrc _
       | Dv_nnrc_impish_core _
       | Dv_nnrc_impish _
+      | Dv_nnrc_imp _
       | Dv_nnrcmr _
       | Dv_cldmr _
       | Dv_dnnrc _
@@ -1758,6 +1842,7 @@ Section CompDriver.
     | L_nnrc => Dv_nnrc Dv_nnrc_stop
     | L_nnrc_impish_core => Dv_nnrc_impish_core Dv_nnrc_impish_core_stop
     | L_nnrc_impish => Dv_nnrc_impish Dv_nnrc_impish_stop
+    | L_nnrc_imp => Dv_nnrc_imp Dv_nnrc_imp_stop
     | L_nnrcmr => Dv_nnrcmr Dv_nnrcmr_stop
     | L_cldmr => Dv_cldmr Dv_cldmr_stop
     | L_dnnrc => Dv_dnnrc Dv_dnnrc_stop
@@ -1843,7 +1928,9 @@ Section CompDriver.
           opc = (get_optim_config L_nnrc config.(comp_optim_config))
         | Dv_nnrc_core (Dv_nnrc_core_to_camp avoid _) =>
           avoid = (List.map fst (vdbindings_of_constants_config config.(comp_constants)))
-        | Dv_nnrc_impish (Dv_nnrc_impish_to_js_ast inputs _) =>
+        | Dv_nnrc_impish (Dv_nnrc_impish_to_nnrc_imp _) =>
+          True (* inputs = (vars_of_constants_config config.(comp_constants)) *)
+        | Dv_nnrc_imp (Dv_nnrc_imp_to_js_ast inputs _) =>
           inputs = (vars_of_constants_config config.(comp_constants))
         | Dv_nnrcmr (Dv_nnrcmr_to_spark_rdd qname _) =>
           qname = config.(comp_qname)
@@ -1918,7 +2005,9 @@ Section CompDriver.
     | Dv_nnrc_impish_core (Dv_nnrc_impish_core_to_nnrc_impish dv) => (L_nnrc_impish_core, Some (Dv_nnrc_impish dv))
     | Dv_nnrc_impish_core (Dv_nnrc_impish_core_stop) => (L_nnrc_impish_core, None)
     | Dv_nnrc_impish (Dv_nnrc_impish_stop) => (L_nnrc_impish, None)
-    | Dv_nnrc_impish (Dv_nnrc_impish_to_js_ast inputs dv) => (L_nnrc_impish, Some (Dv_js_ast dv))
+    | Dv_nnrc_impish (Dv_nnrc_impish_to_nnrc_imp dv) => (L_nnrc_impish, Some (Dv_nnrc_imp dv))
+    | Dv_nnrc_imp (Dv_nnrc_imp_stop) => (L_nnrc_imp, None)
+    | Dv_nnrc_imp (Dv_nnrc_imp_to_js_ast inputs dv) => (L_nnrc_imp, Some (Dv_js_ast dv))
     | Dv_nnrcmr (Dv_nnrcmr_stop) => (L_nnrcmr, None)
     | Dv_nnrcmr (Dv_nnrcmr_to_spark_rdd name dv) => (L_nnrcmr, Some (Dv_spark_rdd dv))
     | Dv_nnrcmr (Dv_nnrcmr_to_nnrc dv) => (L_nnrcmr, Some (Dv_nnrc dv))
@@ -2083,8 +2172,8 @@ Section CompDriver.
       rewrite (constants_config_of_tdbindings_merges t); reflexivity.
   Qed.
 
-  Lemma target_language_of_driver_is_postfix_nnrc_impish:
-    (forall dv, is_postfix_driver (driver_of_language (target_language_of_driver (Dv_nnrc_impish dv))) (Dv_nnrc_impish dv)).
+  Lemma target_language_of_driver_is_postfix_nnrc_imp:
+    (forall dv, is_postfix_driver (driver_of_language (target_language_of_driver (Dv_nnrc_imp dv))) (Dv_nnrc_imp dv)).
   Proof.
     destruct dv; simpl.
     - reflexivity.
@@ -2099,9 +2188,30 @@ Section CompDriver.
                  EmptyString
                  (one_constant_config_of_avoid_list l)
                  EmptyString
-                 nil) (lang:=L_nnrc_impish)
+                 nil) (lang:=L_nnrc_imp)
       ; [eapply target_language_of_driver_is_postfix_js_ast | | ]; simpl; trivial.
       rewrite vars_of_one_constant_config_of_avoid_list; reflexivity.
+  Qed.
+
+
+  Lemma target_language_of_driver_is_postfix_nnrc_impish:
+    (forall dv, is_postfix_driver (driver_of_language (target_language_of_driver (Dv_nnrc_impish dv))) (Dv_nnrc_impish dv)).
+  Proof.
+    destruct dv; simpl.
+    - reflexivity.
+    - rewrite target_language_of_driver_equation
+      ; simpl.
+      eapply is_postfix_plus_one with
+               (config:=mkDvConfig
+                 EmptyString
+                 EmptyString
+                 EmptyString
+                 nil
+                 EmptyString
+                 nil
+                 EmptyString
+                 nil) (lang:=L_nnrc_impish)
+      ; [eapply target_language_of_driver_is_postfix_nnrc_imp | | ]; simpl; trivial.
   Qed.
 
   Lemma target_language_of_driver_is_postfix_nnrc_impish_core:
@@ -2478,6 +2588,7 @@ Section CompDriver.
          target_language_of_driver_is_postfix_nnrc
          target_language_of_driver_is_postfix_nnrc_impish_core
          target_language_of_driver_is_postfix_nnrc_impish
+         target_language_of_driver_is_postfix_nnrc_imp
          target_language_of_driver_is_postfix_nnrcmr
          target_language_of_driver_is_postfix_camp_rule
          target_language_of_driver_is_postfix_tech_rule
@@ -2557,7 +2668,7 @@ Section CompDriver.
         * destruct (H_config (Dv_nnrc (Dv_nnrc_to_java (comp_class_name config0) (comp_java_imports config0) j)));
             try reflexivity.
           rewrite H0; rewrite H3; reflexivity.
-        * destruct (H_config (Dv_nnrc_impish (Dv_nnrc_impish_to_js_ast (vars_of_constants_config (comp_constants config0)) j)));
+        * destruct (H_config (Dv_nnrc_imp (Dv_nnrc_imp_to_js_ast (vars_of_constants_config (comp_constants config0)) j)));
             try reflexivity.
         * destruct (H_config (Dv_nnrcmr (Dv_nnrcmr_to_cldmr (comp_brand_rel config0) c)));
             reflexivity.
@@ -2682,6 +2793,16 @@ Section CompDriver.
           :: L_nnrc_core
           :: L_nnrc_impish_core
           :: nil
+      | L_camp_rule, L_nnrc_imp =>
+        L_camp_rule
+          :: L_camp
+          :: L_nraenv
+          :: L_nraenv
+          :: L_nnrc
+          :: L_nnrc
+          :: L_nnrc_impish
+          :: L_nnrc_imp
+          :: nil
       | L_camp_rule, L_js_ast =>
         L_camp_rule
           :: L_camp
@@ -2690,6 +2811,7 @@ Section CompDriver.
           :: L_nnrc
           :: L_nnrc
           :: L_nnrc_impish
+          :: L_nnrc_imp
           :: L_js_ast
           :: nil
       | L_camp_rule, L_nnrcmr =>
@@ -2860,6 +2982,17 @@ Section CompDriver.
           :: L_nnrc_core
           :: L_nnrc_impish_core
           :: nil
+      | L_tech_rule, L_nnrc_imp =>
+        L_tech_rule
+          :: L_camp_rule
+          :: L_camp
+          :: L_nraenv
+          :: L_nraenv
+          :: L_nnrc
+          :: L_nnrc
+          :: L_nnrc_impish
+          :: L_nnrc_imp
+          :: nil
       | L_tech_rule, L_js_ast =>
         L_tech_rule
           :: L_camp_rule
@@ -2869,6 +3002,7 @@ Section CompDriver.
           :: L_nnrc
           :: L_nnrc
           :: L_nnrc_impish
+          :: L_nnrc_imp
           :: L_js_ast
           :: nil
       | L_tech_rule, L_nnrcmr =>
@@ -3046,6 +3180,17 @@ Section CompDriver.
           :: L_nnrc_core
           :: L_nnrc_impish_core
           :: nil
+      | L_designer_rule, L_nnrc_imp =>
+        L_designer_rule
+          :: L_camp_rule
+          :: L_camp
+          :: L_nraenv
+          :: L_nraenv
+          :: L_nnrc
+          :: L_nnrc
+          :: L_nnrc_impish
+          :: L_nnrc_imp
+          :: nil
       | L_designer_rule, L_js_ast =>
         L_designer_rule
           :: L_camp_rule
@@ -3055,6 +3200,7 @@ Section CompDriver.
           :: L_nnrc
           :: L_nnrc
           :: L_nnrc_impish
+          :: L_nnrc_imp
           :: L_js_ast
           :: nil
       | L_designer_rule, L_nnrcmr =>
@@ -3205,6 +3351,15 @@ Section CompDriver.
           :: L_nnrc_core
           :: L_nnrc_impish_core
           :: nil
+      | L_camp, L_nnrc_imp =>
+        L_camp
+          :: L_nraenv
+          :: L_nraenv
+          :: L_nnrc
+          :: L_nnrc
+          :: L_nnrc_impish
+          :: L_nnrc_imp
+          :: nil
       | L_camp, L_js_ast =>
         L_camp
           :: L_nraenv
@@ -3212,6 +3367,7 @@ Section CompDriver.
           :: L_nnrc
           :: L_nnrc
           :: L_nnrc_impish
+          :: L_nnrc_imp
           :: L_js_ast
           :: nil
       | L_camp, L_nnrcmr =>
@@ -3361,6 +3517,15 @@ Section CompDriver.
           :: L_nnrc_core
           :: L_nnrc_impish_core
           :: nil
+      | L_oql, L_nnrc_imp =>
+        L_oql
+          :: L_nraenv
+          :: L_nraenv
+          :: L_nnrc
+          :: L_nnrc
+          :: L_nnrc_impish
+          :: L_nnrc_imp
+          :: nil
       | L_oql, L_js_ast =>
         L_oql
           :: L_nraenv
@@ -3368,6 +3533,7 @@ Section CompDriver.
           :: L_nnrc
           :: L_nnrc
           :: L_nnrc_impish
+          :: L_nnrc_imp
           :: L_js_ast
           :: nil
       | L_oql, L_nnrcmr =>
@@ -3518,6 +3684,15 @@ Section CompDriver.
           :: L_nnrc_core
           :: L_nnrc_impish_core
           :: nil
+      | L_sql, L_nnrc_imp =>
+        L_sql
+          :: L_nraenv
+          :: L_nraenv
+          :: L_nnrc
+          :: L_nnrc
+          :: L_nnrc_impish
+          :: L_nnrc_imp
+          :: nil
       | L_sql, L_js_ast =>
         L_sql
           :: L_nraenv
@@ -3525,6 +3700,7 @@ Section CompDriver.
           :: L_nnrc
           :: L_nnrc
           :: L_nnrc_impish
+          :: L_nnrc_imp
           :: L_js_ast
           :: nil
       | L_sql, L_nnrcmr =>
@@ -3675,6 +3851,15 @@ Section CompDriver.
           :: L_nnrc_core
           :: L_nnrc_impish_core
           :: nil
+      | L_sqlpp, L_nnrc_imp =>
+        L_sqlpp
+          :: L_nraenv
+          :: L_nraenv
+          :: L_nnrc
+          :: L_nnrc
+          :: L_nnrc_impish
+          :: L_nnrc_imp
+          :: nil
       | L_sqlpp, L_js_ast =>
         L_sqlpp
           :: L_nraenv
@@ -3682,6 +3867,7 @@ Section CompDriver.
           :: L_nnrc
           :: L_nnrc
           :: L_nnrc_impish
+          :: L_nnrc_imp
           :: L_js_ast
           :: nil
       | L_sqlpp, L_nnrcmr =>
@@ -3832,6 +4018,15 @@ Section CompDriver.
           :: L_nnrc_core
           :: L_nnrc_impish_core
           :: nil
+      | L_lambda_nra, L_nnrc_imp =>
+        L_lambda_nra
+          :: L_nraenv
+          :: L_nraenv
+          :: L_nnrc
+          :: L_nnrc
+          :: L_nnrc_impish
+          :: L_nnrc_imp
+          :: nil
       | L_lambda_nra, L_js_ast =>
         L_lambda_nra
           :: L_nraenv
@@ -3839,6 +4034,7 @@ Section CompDriver.
           :: L_nnrc
           :: L_nnrc
           :: L_nnrc_impish
+          :: L_nnrc_imp
           :: L_js_ast
           :: nil
       | L_lambda_nra, L_nnrcmr =>
@@ -3983,6 +4179,16 @@ Section CompDriver.
           :: L_nnrc_core
           :: L_nnrc_impish_core
           :: nil
+      | L_nra, L_nnrc_imp =>
+        L_nra
+          :: L_nraenv_core
+          :: L_nraenv
+          :: L_nraenv
+          :: L_nnrc
+          :: L_nnrc
+          :: L_nnrc_impish
+          :: L_nnrc_imp
+          :: nil
       | L_nra, L_js_ast =>
         L_nra
           :: L_nraenv_core
@@ -3991,6 +4197,7 @@ Section CompDriver.
           :: L_nnrc
           :: L_nnrc
           :: L_nnrc_impish
+          :: L_nnrc_imp
           :: L_js_ast
           :: nil
       | L_nra, L_nnrcmr =>
@@ -4135,6 +4342,15 @@ Section CompDriver.
           :: L_nnrc_core
           :: L_nnrc_impish_core
           :: nil
+      | L_nraenv_core, L_nnrc_imp =>
+        L_nraenv_core
+          :: L_nraenv
+          :: L_nraenv
+          :: L_nnrc
+          :: L_nnrc
+          :: L_nnrc_impish
+          :: L_nnrc_imp
+          :: nil
       | L_nraenv_core, L_js_ast =>
         L_nraenv_core
           :: L_nraenv
@@ -4142,6 +4358,7 @@ Section CompDriver.
           :: L_nnrc
           :: L_nnrc
           :: L_nnrc_impish
+          :: L_nnrc_imp
           :: L_js_ast
           :: nil
       | L_nraenv_core, L_nnrcmr =>
@@ -4279,12 +4496,21 @@ Section CompDriver.
           :: L_nnrc_core
           :: L_nnrc_impish_core
           :: nil
+      | L_nraenv, L_nnrc_imp =>
+        L_nraenv
+          :: L_nraenv
+          :: L_nnrc
+          :: L_nnrc
+          :: L_nnrc_impish
+          :: L_nnrc_imp
+          :: nil
       | L_nraenv, L_js_ast =>
         L_nraenv
           :: L_nraenv
           :: L_nnrc
           :: L_nnrc
           :: L_nnrc_impish
+          :: L_nnrc_imp
           :: L_js_ast
           :: nil
       | L_nraenv, L_nnrcmr =>
@@ -4404,11 +4630,19 @@ Section CompDriver.
           :: L_nnrc_core
           :: L_nnrc_impish_core
           :: nil
+      | L_nnrc_core, L_nnrc_imp =>
+        L_nnrc_core
+          :: L_nnrc
+          :: L_nnrc
+          :: L_nnrc_impish
+          :: L_nnrc_imp
+          :: nil
       | L_nnrc_core, L_js_ast =>
         L_nnrc_core
           :: L_nnrc
           :: L_nnrc
           :: L_nnrc_impish
+          :: L_nnrc_imp
           :: L_js_ast
           :: nil
       | L_nnrc_core, L_nnrcmr =>
@@ -4526,10 +4760,17 @@ Section CompDriver.
           :: L_nnrc_core
           :: L_nnrc_impish_core
           :: nil
+      | L_nnrc, L_nnrc_imp =>
+        L_nnrc
+          :: L_nnrc
+          :: L_nnrc_impish
+          :: L_nnrc_imp
+          :: nil
       | L_nnrc, L_js_ast =>
         L_nnrc
           :: L_nnrc
           :: L_nnrc_impish
+          :: L_nnrc_imp
           :: L_js_ast
           :: nil
       | L_nnrc, L_nnrcmr =>
@@ -4584,12 +4825,18 @@ Section CompDriver.
       | L_nnrc_impish, L_nnrc_impish =>
         L_nnrc_impish
           :: nil
+      | L_nnrc_impish, L_nnrc_imp =>
+        L_nnrc_impish
+          :: L_nnrc_imp
+          :: nil
       | L_nnrc_impish, L_js_ast =>
         L_nnrc_impish
+          :: L_nnrc_imp
           :: L_js_ast
           :: nil
       | L_nnrc_impish, L_javascript =>
         L_nnrc_impish
+          :: L_nnrc_imp
           :: L_js_ast
           :: L_javascript
           :: nil
@@ -4601,14 +4848,34 @@ Section CompDriver.
         L_nnrc_impish_core
           :: L_nnrc_impish
           :: nil
+      | L_nnrc_impish_core, L_nnrc_imp =>
+        L_nnrc_impish_core
+          :: L_nnrc_impish
+          :: L_nnrc_imp
+          :: nil
       | L_nnrc_impish_core, L_js_ast =>
         L_nnrc_impish_core
           :: L_nnrc_impish
+          :: L_nnrc_imp
           :: L_js_ast
           :: nil
       | L_nnrc_impish_core, L_javascript =>
         L_nnrc_impish_core
           :: L_nnrc_impish
+          :: L_nnrc_imp
+          :: L_js_ast
+          :: L_javascript
+          :: nil
+      (* From nnrc_impish: *)
+      | L_nnrc_imp, L_nnrc_imp =>
+        L_nnrc_imp
+          :: nil
+      | L_nnrc_imp, L_js_ast =>
+        L_nnrc_imp
+          :: L_js_ast
+          :: nil
+      | L_nnrc_imp, L_javascript =>
+        L_nnrc_imp
           :: L_js_ast
           :: L_javascript
           :: nil
@@ -4680,12 +4947,21 @@ Section CompDriver.
           :: L_nnrc_core
           :: L_nnrc_impish_core
           :: nil
+      | L_nnrcmr, L_nnrc_imp =>
+        L_nnrcmr
+          :: L_nnrcmr
+          :: L_nnrc
+          :: L_nnrc
+          :: L_nnrc_impish
+          :: L_nnrc_imp
+          :: nil
       | L_nnrcmr, L_js_ast =>
         L_nnrcmr
           :: L_nnrcmr
           :: L_nnrc
           :: L_nnrc
           :: L_nnrc_impish
+          :: L_nnrc_imp
           :: L_js_ast
           :: nil
       | L_nnrcmr, L_javascript =>
@@ -4894,6 +5170,15 @@ Section CompDriver.
     Qed.
 
     Hint Resolve exists_path_from_source_target_completeness_js_ast : exists_path_hints.
+
+    Lemma exists_path_from_source_target_completeness_nnrc_imp :
+      (forall dv,
+          exists_path_from_source_target L_nnrc_imp (target_language_of_driver (Dv_nnrc_imp dv))).
+    Proof.
+      destruct dv; prove_exists_path_complete.
+    Qed.
+
+    Hint Resolve exists_path_from_source_target_completeness_nnrc_imp : exists_path_hints.
 
     Lemma exists_path_from_source_target_completeness_nnrc_impish :
       (forall dv,
